commit

Projects/Esolangs/Cornucopia/Basic.lean
@@ -2,303 +2,6 @@ import Projects.Esolangs.Cornucopia.Defs
 
 attribute [-simp] List.getElem!_eq_getElem?_getD
 
-section logic
-
-@[simp] theorem or_iff_or_left {p q r : Prop} : (p ∨ q ↔ p ∨ r) ↔ ¬p → (q ↔ r) := by tauto
-@[simp] theorem or_iff_or_right {p q r : Prop} : (p ∨ q ↔ r ∨ q) ↔ ¬q → (p ↔ r) := by tauto
-@[simp] theorem imp_not_imp_iff {p q : Prop} : p → ¬p → q ↔ True := by tauto
-@[simp] theorem not_imp_imp_iff {p q : Prop} : ¬p → p → q ↔ True := by tauto
-
--- #check 0 #exit
-
-end logic
-
-namespace List
-
-variable {α β γ : Type*}
-variable {xs ys zs : List α}
-
-@[simp]
-theorem length_mkList {n} {f : ℕ → α} : (mkList n f).length = n := by
-  simp [mkList]
-
-@[simp]
-theorem mem_mkList {n} {f : ℕ → α} {x} : x ∈ mkList n f ↔ ∃ i < n, f i = x := by
-  simp [mkList]
-
-theorem mergeSort_eq_mergeSort_iff {le : α → α → Bool}
-(trans : ∀ (a b c : α), le a b → le b c → le a c)
-(total : ∀ (a b : α), le a b || le b a)
-(antisymm : ∀ (a b : α), le a b → le b a → a = b) :
-xs.mergeSort le = ys.mergeSort le ↔ xs.Perm ys := by
-  use perm_of_mergeSort_eq_mergeSort
-  intro h
-  apply eq_of_perm_of_pairwise (r := (le · ·))
-  · simpa
-  · apply pairwise_mergeSort trans total
-  · apply pairwise_mergeSort trans total
-  · grind
-  · grind
-  · grind
-
-@[simp]
-theorem map_mkList {n} {f : ℕ → α} {g : α → β} :
-(mkList n f).map g = mkList n λ i => g (f i) := by
-  simp [mkList]
-
-@[simp]
-theorem getElem_mkList {n} {f : ℕ → α} {i}
-{h : i < (mkList n f).length} : (mkList n f)[i] = f i := by
-  simp [mkList]
-
-@[simp]
-theorem mkList_length_getElem! [ha : Inhabited α] : mkList xs.length (xs[·]!) = xs := by
-  simp [mkList]
-
--- #check 0 #exit
-
-end List
-
-namespace Std.ExtDHashMap
-
-open Std
-
-variable {α : Type*} {β : α → Type*} {γ : α → Type*}
-variable [hh₁ : DecidableEq α] [hh₂ : Hashable α]
-variable {mp mp₁ mp₂ m m₁ m₂ m₃ : ExtDHashMap α β}
-variable [ha : LinearOrder α]
-omit ha
-
-attribute [simp] keys_empty
-
-include ha in
-theorem toList_insert_of_not_mem {i x} (h : i ∉ m) : (m.insert i x).toList =
-(⟨i, x⟩ :: m.toList).mergeSort (·.1 ≤ ·.1) := by
-  rw [List.eq_iff_of_nodup_and_pairwise (r := (·.1 ≤ ·.1))]
-  rotate_left
-  · simp
-  · simp [get?_eq_none_of_not_mem h]
-  · rintro ⟨j, y⟩ ⟨k, z⟩
-    simp; grind
-  · simp
-  · have h₁ := @List.pairwise_mergeSort
-    specialize @h₁ ((i : α) × β i) (le := (·.1 ≤ ·.1))
-      (by simp) (by simp) (⟨i, x⟩ :: m.toList)
-    grind
-  rintro ⟨j, y⟩; simp
-  by_cases h₁ : j = i
-  · subst h₁; simp [eq_comm, get?_eq_none_of_not_mem h]
-  simp [h₁, get?_insert, ne_symm' h₁]
-
-include ha in
-theorem keys_insert_of_not_mem {i x} (h : i ∉ m) :
-(m.insert i x).keys = (i :: m.keys).mergeSort := by
-  simp [keys_eq_map_fst_toList, toList_insert_of_not_mem h]
-  apply List.eq_of_sortedLE_and_perm
-  · rw [List.map_mergeSort (s := (· ≤ ·)) (by simp)]
-    apply List.sortedLE_mergeSort
-  · apply List.sortedLE_mergeSort
-  simp
-  rw [List.perm_iff_mem_iff_of_nodup]; simp
-  on_goal 2 => simpa [←keys_eq_map_fst_toList]
-  rw [List.nodup_map_iff_inj_on]
-  rotate_left
-  · simp [get?_eq_none_of_not_mem h]
-  simp
-  split_ands
-  · rintro ⟨j, y⟩ h₁ rfl
-    simp [get?_eq_none_of_not_mem h] at h₁
-  rintro ⟨j, y⟩ h₁
-  dsimp at h₁ ⊢
-  split_ands
-  · rintro rfl; simp [get?_eq_none_of_not_mem h] at h₁
-  · grind
-
-@[simp]
-theorem get?_out_inner {i} : m.inner.out.get? i = m.get? i := by
-  rcases m with ⟨m⟩
-  induction m using Quotient.inductionOn
-  simp [get?, lift]
-
-@[simp]
-theorem get?_mk {m i} : ({inner := m} : ExtDHashMap α β).get? i = m.out.get? i := by
-  simp [get?, lift, Quotient.lift_eq]
-
-@[simp]
-theorem insert_mk {m i x} :
-({inner := m} : ExtDHashMap α β).insert i x = {inner := ⟦m.out.insert i x⟧} := by
-  simp [insert, lift, Quotient.lift_eq]
-
-@[simp]
-theorem erase_mk {m i} :
-({inner := m} : ExtDHashMap α β).erase i = {inner := ⟦m.out.erase i⟧} := by
-  simp [erase, lift, Quotient.lift_eq]
-
-@[simp]
-theorem insert_erase_eq_self_iff {i x} :
-(m.erase i).insert i x = m ↔ m.get? i = some x := by
-  constructor <;> intro h
-  · rw [←h]; simp
-  rw [ext_iff']
-  have h₁ := @DHashMap.insert_erase_equiv
-  specialize @h₁ α β _ _ m.inner.out i x _
-  · simpa
-  symm; apply h₁.symm.trans; symm; clear h₁
-  change (_ : DHashMap α β) ≈ _
-  rw [←Quotient.eq_mk_iff_out]
-  rcases m with ⟨m⟩
-  simp at h ⊢
-  apply DHashMap.equiv_iff_get?.mpr
-  intro j
-  ext y
-  simp [DHashMap.get?_insert]
-
-include ha in @[simp]
-theorem keys_eq_keys_iff {m₁ : ExtDHashMap α β} {m₂ : ExtDHashMap α γ} :
-m₁.keys = m₂.keys ↔ ∀ i, i ∈ m₁ ↔ i ∈ m₂ := by
-  induction m₂ using ind generalizing m₁
-  · simp [eq_empty_iff]
-  nm m₂ i x h₁ ih
-  simp
-  rw [keys_insert_of_not_mem h₁]
-  constructor
-  · intro h₂ j
-    replace h₂ := congrArg (j ∈ ·) h₂
-    simp at h₂
-    tauto
-  intro h₂
-  have h₃ : i ∈ m₁; grind
-  clear x
-  obtain ⟨x, h₄⟩ := get?_eq_some_of_mem h₃
-  have h₅ : m₁ = (m₁.erase i).insert i x
-  · symm; simpa
-  rw [h₅]
-  rw [keys_insert_of_not_mem (by simp)]
-  rw [List.mergeSort_eq_mergeSort_iff (by simp) (by simp) (by simp)]
-  simp; rw [List.perm_iff_mem_iff_of_nodup (by simp) (by simp)]; grind
-
--- #check 0 #exit
-
-end Std.ExtDHashMap
-
-namespace Map
-
-open Std
-
-universe u v w
-variable {α : Type u} {β : Type v} {γ : Type w}
-variable [hh₁ : DecidableEq α] [hh₂ : Hashable α]
-variable {mp m m₁ m₂ m₃ : Map α β}
-variable [ha : LinearOrder α]
-omit ha
-
-theorem get!_insert [hb : Inhabited β] {i x j} :
-(mp.insert i x).get! j = if j = i then x else mp.get! j := by
-  simp [get!_eq_get!_get?, get?_insert]; grind
-
-theorem get?_ofList_eq_some_iff {xs : List (α × β)} {i x}
-(h : (xs.map (·.1)).Nodup) : (ofList xs).get? i = some x ↔ ⟨i, x⟩ ∈ xs := by
-  simp [ofList]; rw [ExtDHashMap.get?_ofList_eq_some_iff (by simpa)]; simp
-
-theorem get?_ofList_of_nodup {xs : List (α × β)} {i} (h : (xs.map (·.1)).Nodup) :
-(ofList xs).get? i = (xs.find? (·.fst = i)).map (·.2) := by
-  unfold Option.map; split
-  · nm a x h₁; clear a
-    rename' i => j
-    rcases x with ⟨i, x⟩
-    rw [get?_ofList_eq_some_iff h]
-    grind
-  nm a h₁; clear a
-  simp at h₁ ⊢
-  grind
-
-theorem get!_ofList_of_nodup [hb : Inhabited β] {xs : List (α × β)} {i}
-(h : (xs.map (·.1)).Nodup) : (ofList xs).get! i =
-((xs.find? (·.fst = i)).map (·.2)).get! := by
-  rw [get!_eq_get!_get?, get?_ofList_of_nodup h]
-
-@[simp]
-theorem mem_union {i} : i ∈ m₁ ∪ m₂ ↔ i ∈ m₁ ∨ i ∈ m₂ := by
-  simp [mem_iff_get?_eq_some, get?_union]; grind
-
-include ha in @[simp]
-theorem keys_mk {mp} : (⟨mp⟩ : Map α β).keys = mp.keys := rfl
-
-@[simp]
-theorem insert_mk {m i x} : (⟨m⟩ : Map α β).insert i x = ⟨m.insert i x⟩ := rfl
-
-@[simp]
-theorem erase_mk {m i} : (⟨m⟩ : Map α β).erase i = ⟨m.erase i⟩ := rfl
-
-include ha in
-theorem toList_insert_of_not_mem {i x} (h : i ∉ m) : (m.insert i x).toList =
-(⟨i, x⟩ :: m.toList).mergeSort (·.1 ≤ ·.1) := by
-  rcases m with ⟨m⟩; simp at h ⊢
-  rw [ExtDHashMap.toList_insert_of_not_mem h]
-  rw [List.map_mergeSort (s := (·.1 ≤ ·.1)) (by simp)]
-  simp
-
-include ha in
-theorem keys_insert_of_not_mem {i x} (h : i ∉ m) :
-(m.insert i x).keys = (i :: m.keys).mergeSort := by
-  rcases m with ⟨m⟩; simp at h ⊢
-  rw [ExtDHashMap.keys_insert_of_not_mem h]
-
-@[simp]
-theorem insert_erase_eq_self_iff {i x} :
-(m.erase i).insert i x = m ↔ m.get? i = some x := by
-  rcases m with ⟨m⟩; simp
-
-include ha in @[simp]
-theorem keys_eq_keys_iff {m₁ : Map α β} {m₂ : Map α γ} :
-m₁.keys = m₂.keys ↔ ∀ i, i ∈ m₁ ↔ i ∈ m₂ := by
-  rcases m₁, m₂ with ⟨⟨m₁⟩, ⟨m₂⟩⟩; simp
-
-theorem union_assoc : (m₁ ∪ m₂) ∪ m₃ = m₁ ∪ (m₂ ∪ m₃) := by
-  simp [ext_iff, get?_union]; grind
-
-@[simp]
-theorem union_self : m ∪ m = m := by
-  simp [ext_iff, get?_union]
-
-@[simp]
-theorem union_union_self : m₁ ∪ (m₁ ∪ m₂) = m₁ ∪ m₂ := by
-  simp [←union_assoc]
-
-def diff (m₁ m₂ : Map α β) : Map α β :=
-  ⟨m₁.1 \ m₂.1⟩
-
-instance : SDiff (Map α β) := ⟨diff⟩
-theorem diff_def : m₁ \ m₂ = m₁.diff m₂ := rfl
-
-@[simp]
-theorem mk_diff_mk {m₁ m₂} : (⟨m₁⟩ : Map α β) \ ⟨m₂⟩ = ⟨m₁ \ m₂⟩ := rfl
-
-theorem get?_diff {i} : (m₁ \ m₂).get? i = if i ∈ m₂ then none else m₁.get? i := by
-  rcases m₁, m₂ with ⟨⟨m₁⟩, ⟨m₂⟩⟩; simp [ExtDHashMap.get?_diff]
-
-@[simp]
-theorem union_diff_self : m₁ ∪ (m₂ \ m₁) = m₂ ∪ m₁ := by
-  simp [ext_iff, get?_union, get?_diff]
-  intro i
-  rw! (castMode := .all) [mem_iff_get?_eq_some]
-  split_ifs with h; grind
-  simp at h
-  rw [←Option.eq_none_iff_forall_ne_some] at h
-  grind
-
-theorem union_eq_self_left_iff : m₁ ∪ m₂ = m₁ ↔
-∀ i x, m₂.get? i = some x → m₁.get? i = some x := by
-  simp [ext_iff, get?_union, Option.or]; grind
-
-@[simp]
-theorem union_insert_empty {i x} : m₁ ∪ (∅ : Map α β).insert i x = m₁.insert i x := by
-  simp [ext_iff, get?_union, get?_insert]; grind
-
--- #check 0 #exit
-
-end Map
-
 namespace Esolangs.Cornucopia
 
 structure CompatibleDefs (defs : Map String Def) (fs : Map String (List ℕ → ℕ)) : Prop where
@@ -315,20 +18,6 @@ structure WFDefs (defs : List (String × Def)) : Prop where
   wf_main : ∃ d, (mainName, d) ∈ defs ∧ d.arity = 1
   wf_def ⦃name d⦄ : (name, d) ∈ defs → d.WF (Prog.ofDefs defs)
   exiu_compatible : ∃! fs, CompatibleDefs (.ofList defs) fs
-
--- #check 0 #exit
-
-def exprId : Expr :=
-  .arg 0
-
-def exprLoop (name : String) : Expr :=
-  .call name [.arg 0]
-
-def progId : Prog :=
-  .ofDefs [(mainName, ⟨1, exprId⟩)]
-
-def progLoop : Prog :=
-  .ofDefs [(mainName, ⟨1, exprLoop mainName⟩)]
 
 -- #check 0 #exit
 
@@ -369,17 +58,6 @@ theorem arity_ofDefs {defs name} (h : ¬IsBuiltin name) :
 @[simp]
 theorem Prog.main_ofDefs {xs} : (Prog.ofDefs xs).main = (Map.ofList xs).get! mainName := by
   simp [ofDefs]; rw [Map.get!_union_right]; simp
-
-@[simp]
-theorem main_progId : progId.main = ⟨1, exprId⟩ := by
-  simp [progId, Map.get!_insert]
-
-@[simp]
-theorem main_progLoop : progLoop.main = ⟨1, exprLoop mainName⟩ := by
-  simp [progLoop, Map.get!_insert]
-
-@[simp] theorem wf_exprId {prog} : exprId.WF prog 1 := by simp [Expr.WF, exprId]
-@[simp] theorem wf_defId : (Def.mk 1 (.arg 0)).WF progId := wf_exprId
 
 @[simp]
 theorem Expr.run_arg {i prog f args} : (arg i).eval prog f args = args[i]! := by
@@ -581,14 +259,16 @@ theorem Builtin.eval_of_ne_arity {b : Builtin} {xs}
 (h : xs.length ≠ b.arity) : b.eval xs = 0 := by
   simp at h ⊢; simp [Builtin.eval, fn, h]
 
-theorem CompatibleDefs.get?_builtin {defs fs} {b : Builtin} (H : WFDefs defs)
-(H₁ : CompatibleDefs (.ofList defs) fs) : (builtinFs ∪ fs).get? b.name = some b.eval := by
+theorem CompatibleDefs.get?_builtin {defs fs} (H : WFDefs defs)
+(H₁ : CompatibleDefs (.ofList defs) fs) (b : Builtin) :
+(builtinFs ∪ fs).get? b.name = some b.eval := by
   have h₃ := H₁.keys_fs; simp at h₃
   rw [Map.get?_union_left]; simp
   simp [h₃]; intro d; apply H.builtin_not_mem_defs
 
-theorem CompatibleDefs.get!_builtin {defs fs} {b : Builtin} (H : WFDefs defs)
-(H₁ : CompatibleDefs (.ofList defs) fs) : (builtinFs ∪ fs).get! b.name = b.eval := by
+theorem CompatibleDefs.get!_builtin {defs fs} (H : WFDefs defs)
+(H₁ : CompatibleDefs (.ofList defs) fs) (b : Builtin) :
+(builtinFs ∪ fs).get! b.name = b.eval := by
   simp [Map.get!_eq_get!_get?, H₁.get?_builtin H]
 
 @[simp]
@@ -613,218 +293,140 @@ theorem Builtin.name_ne_mainName {b : Builtin} : b.name ≠ mainName := by
 theorem Builtin.mainName_ne_name {b : Builtin} : mainName ≠ b.name :=
   ne_symm' b.name_ne_mainName
 
--- #check 0 #exit
+theorem Prog.Compatible.builtinFs_union {defs fs}
+(H : (Prog.ofDefs defs).Compatible fs) : fs ∪ builtinFs = fs := by
+  rw [Map.union_eq_self_left_iff]
+  intro name f h
+  simp at h
+  obtain ⟨b, rfl, rfl⟩ := h
+  exact H.get?_builtin
 
--- theorem Prog.Compatible.get?_builtin_ofDefs {defs} {b : Builtin} {fs}
--- (H₁ : (Prog.ofDefs defs).Compatible fs) : fs.get? b.name = some b.eval := by
---   have h₁ := @H₁.eval_eq b.name
---   specialize @h₁ (by simp) (mkList b.arity id) _
---   ·
---     clear h₁
---     cases H
---     simp [arity, H.def_builtin]
+theorem WFDefs.get?_fs_of_mem_defs {defs fs name d} (H : WFDefs defs)
+(h : (name, d) ∈ defs) : (builtinFs ∪ fs).get? name = fs.get? name := by
+  simp [Map.get?_union_right, H.not_isBuiltin_of_mem h]
 
--- #check 0 #exit
+theorem WFDefs.get!_fs_of_mem_defs {defs fs name d} (H : WFDefs defs)
+(h : (name, d) ∈ defs) : (builtinFs ∪ fs).get! name = fs.get! name := by
+  simp [Map.get!_eq_get!_get?, H.get?_fs_of_mem_defs h]
 
--- theorem Prog.Compatible.builtinFs_union {defs fs} (H : (Prog.ofDefs defs).WF)
--- (H₁ : (Prog.ofDefs defs).Compatible fs) : fs ∪ builtinFs = fs := by
---   rw [Map.union_eq_self_left_iff]
---   intro name f h
---   simp at h
---   obtain ⟨b, rfl, rfl⟩ := h
---   exact H₁.get?_builtin H
+theorem WFDefs.get?_of_mem_defs' {defs} (H : WFDefs defs) {name d}
+(h : (name, d) ∈ defs) : (Map.ofList defs).get? name = some d := by
+  rwa [Map.get?_ofList_eq_some_iff H.nodup_names]
 
-example : ¬∀ {defs} (H : WFDefs defs),
-∃! fs, (Prog.ofDefs defs).Compatible fs := by
-  simp [not_exiu_iff]
-  use [(mainName, ⟨1, exprId⟩)]
-  split_ands
-  ·
-    constructor <;> simp
-    use .ofList [(mainName, fn 1 (·[0]!))]
+theorem WFDefs.toList_defs {defs} (H : WFDefs defs) :
+(Map.ofList defs).toList = defs.mergeSort (·.1 ≤ ·.1) :=
+  Map.toList_ofList H.nodup_names
+
+theorem Prog.Compatible.union_builtinFs {prog : Prog} {fs}
+(H : prog.Compatible fs) : fs ∪ builtinFs = fs := by
+  have h₁ := @H.get?_builtin
+  ext name : 1
+  rw [Map.get?_union_ite]
+  simp
+  rintro ⟨b, rfl⟩
+  simp [h₁]
+
+theorem Prog.Compatible.fs_eq_union {prog : Prog} {fs} (H : prog.Compatible fs) :
+∃ fs', fs = builtinFs ∪ fs' ∧ ∀ (b : Builtin), b.name ∉ fs' := by
+  use fs \ builtinFs; simp [H.union_builtinFs]
+
+theorem CompatibleDefs.builtin_not_mem {defs fs} (H : WFDefs defs)
+(H₁ : CompatibleDefs (.ofList defs) fs) (b : Builtin) : b.name ∉ fs := by
+  have h₁ := congrArg (b.name ∈ ·) H₁.keys_fs
+  simp at h₁; simp [h₁]; intro d; exact H.not_mem_builtin
+
+@[simp] theorem Builtin.eval_succ : Builtin.succ.eval = fn 1 (·[0]! + 1) := rfl
+@[simp] theorem Builtin.eval_sub : Builtin.sub.eval = fn 2 (λ xs => xs[0]! - xs[1]!) := rfl
+
+theorem WFDefs.compatible_fs_aux₁ {defs fs} (H : WFDefs defs)
+(H₁ : CompatibleDefs (Map.ofList defs) fs) :
+(Prog.ofDefs defs).Compatible (builtinFs ∪ fs) := by
+  constructor
+  · simp
+    intro name h₁
+    have h₂ := H₁.keys_fs
+    simp at h₂
+    apply h₂
+  · intro b; simp [H₁.get?_builtin H]
+  · intro name h₁ xs h₂
+    simp at h₁
+    have h₃ := H₁.keys_fs
+    simp at h₃
+    specialize h₃ name
+    rw [←h₃] at h₁
+    rcases h₁ with ⟨b, rfl⟩ | h₁
+    · rw [H₁.get!_builtin H]
+      rw [H.arity_builtin] at h₂
+      exact b.eval_of_ne_arity h₂
+    rw [h₃] at h₁
+    choose d h₁ using h₁
+    rw [H.arity_of_mem_defs h₁] at h₂
+    have h₄ := @H₁.eval_of_ne_arity name
+    specialize @h₄ d (H.get?_of_mem_defs' h₁) xs h₂
+    rwa [Map.get!_union_right]
+    simp [H.not_isBuiltin_of_mem h₁]
+  · intro name h₁ xs h₂
+    simp at h₁
+    have h₃ := H₁.keys_fs
+    simp at h₃
+    rcases h₁ with ⟨b, rfl⟩ | ⟨d, h₁⟩
+    · rw [H₁.get!_builtin H]
+      simp [H.arity_builtin] at h₂
+      rw [H.expr_builtin]
+      simp [Builtin.eval, fn, h₂, Builtin.expr, Expr.eval, H₁.get!_builtin H]
+      simp [←h₂]
+    · symm
+      rw [H.get!_fs_of_mem_defs h₁, H.expr_of_mem_defs h₁]
+      have h₄ := @H₁.eval_eq
+      rw [H.arity_of_mem_defs h₁] at h₂
+      specialize @h₄ name d (H.get?_of_mem_defs' h₁) xs h₂
+      rw [h₄]; clear h₄
+      congr 1
+      simp [Prog.ofDefs]
+
+theorem WFDefs.compatible_fs_aux₂ {defs fs'} (H : WFDefs defs)
+(H₂ : (Prog.ofDefs defs).Compatible (builtinFs ∪ fs'))
+(h : ∀ (b : Builtin), b.name ∉ fs') :
+CompatibleDefs (.ofList defs) fs' := by
+  constructor
+  · have h₁ := H₂.keys_fs
+    simp [IsBuiltin] at h₁
     simp
-    split_ands
-    ·
-      constructor <;> simp [Map.get?_insert, Map.get!_eq_get!_get?, fn, exprId]
-    ·
-      intro fs
-      rintro ⟨h₁, h₂, h₃⟩
-      simp [Map.get?_insert, Map.get!_eq_get!_get?, exprId] at h₁ h₂ h₃
-      simp [Map.ext_iff, Map.get?_insert]
-      intro name
-      rw! (castMode := .all) [eq_comm (a := mainName)]
-      split_ifs with h₄
-      rotate_left
-      ·
-        simp [←h₁] at h₄
-        simpa
-      subst h₄
-      specialize h₁ mainName
-      simp at h₁
-      rw [Map.mem_iff_get?_eq_some] at h₁
-      choose f h₁ using h₁
-      ext xs
-      simp [h₁]
-      unfold fn
-      simp
-      revert xs
-      simp
-      ext xs
-      split_ifs with h₄
-      ·
-        specialize h₃ h₄
-        simp [h₁] at h₃
-        rw [h₃]
-      ·
-        specialize h₂ h₄
-        simp [h₁] at h₂
-        rw [h₂]
-  
-  intro fs h
-  use fs.insert Builtin.succ.name # fn 1 # λ xs =>
-    fs.get! Builtin.succ.name xs + 1
-  split_ands
-  ·
-    obtain ⟨h₂, h₃, h₄⟩ := h
-    simp at h₂ h₃ h₄
-    constructor <;> simp
-    ·
-      intro name
-      simp [h₂]
-      rintro rfl
-      simp
-    ·
-      rintro name (⟨b, rfl⟩ | rfl) xs h
-      ·
-        specialize @h₃ b.name (by simp) xs h
-        simp [Prog.arity, Prog.ofDefs, Map.get!_insert] at h
-        simp [Map.get!_insert]
-        split_ifs with h₅
-        · subst h₅
-          simp at h
-          simp [fn, h]
-        · exact h₃
-      ·
-        simp [Map.get!_insert]
-        exact h₃ (by simp) h
-    ·
-      rintro name (⟨b, rfl⟩ | rfl) xs h
-      ·
-        simp [Map.get!_insert, Prog.expr, Prog.ofDefs] at h ⊢
-        split_ifs with h₅
-        ·
-          subst h₅
-          simp at h
-          simp [fn, h, Builtin.expr, Expr.eval, Map.get!_insert]
-          rw [←h]; simp
-        ·
-          simp [Builtin.expr, Expr.eval, Map.get!_insert, h₅, ←h]
-      ·
-        specialize @h₄ mainName (by simp) xs h
-        simp [Map.get!_insert, Prog.expr, Prog.ofDefs] at h ⊢
-        simp [exprId]
-        rw [h₄]
-        simp [Prog.ofDefs, Map.get!_insert, exprId]
-  
-  ·
-    apply ne_of_congr (·.get! Builtin.succ.name)
-    simp [Map.get!_insert, funext_iff]
-    use [0]
-    simp [fn]
-
-#check 0 #exit
+    intro name
+    specialize h₁ name
+    use by grind
+    rintro ⟨d, h₂⟩
+    specialize h₁ _
+    · rintro b rfl
+      replace h₂ := H.not_isBuiltin_of_mem h₂
+      simp at h₂
+    grind
+  · intro name d h₁ xs h₂
+    rw [Map.get?_ofList_eq_some_iff H.nodup_names] at h₁
+    have h₃ := @H₂.eval_of_ne_arity
+    specialize @h₃ name (by simp; tauto) xs (by simpa [H.arity_of_mem_defs h₁])
+    rwa [Map.get!_union_right # by simp [H.not_isBuiltin_of_mem h₁]] at h₃
+  · intro name d h₁ xs h₂
+    rw [Map.get?_ofList_eq_some_iff H.nodup_names] at h₁
+    have h₃ := @H₂.eval_eq
+    specialize @h₃ name (by simp; tauto) xs (by simpa [H.arity_of_mem_defs h₁])
+    rw [Map.get!_union_right # by simp [H.not_isBuiltin_of_mem h₁]] at h₃
+    rw [h₃]; clear h₃
+    simp [H.expr_of_mem_defs h₁]
+    congr 1
 
 theorem WFDefs.compatible_fs {defs} (H : WFDefs defs) :
 ∃! fs, (Prog.ofDefs defs).Compatible fs := by
   obtain ⟨fs, H₁, H₂⟩ := H.exiu_compatible
   dsimp at H₂
   use builtinFs ∪ fs
-  dsimp; split_ands
-  · constructor
-    ·
-      simp
-      intro name h₁
-      have h₂ := H₁.keys_fs
-      simp at h₂
-      apply h₂
-    · intro name h₁ xs h₂
-      simp at h₁
-      have h₃ := H₁.keys_fs
-      simp at h₃
-      specialize h₃ name
-      rw [←h₃] at h₁
-      rcases h₁ with ⟨b, rfl⟩ | h₁
-      · rw [H₁.get!_builtin H]
-        rw [H.arity_builtin] at h₂
-        exact b.eval_of_ne_arity h₂
-      rw [h₃] at h₁
-      choose d h₁ using h₁
-      rw [H.arity_of_mem_defs h₁] at h₂
-      have h₄ := @H₁.eval_of_ne_arity name
-      specialize @h₄ d _ xs h₂
-      · rwa [Map.get?_ofList_eq_some_iff H.nodup_names]
-      rwa [Map.get!_union_right]
-      simp [H.not_isBuiltin_of_mem h₁]
-    ·
-      intro name h₁ xs h₂
-      simp at h₁
-      have h₃ := H₁.keys_fs
-      simp at h₃
-      rcases h₁ with ⟨b, rfl⟩ | ⟨d, h₁⟩
-      ·
-        rw [H₁.get!_builtin H]
-        simp [H.arity_builtin] at h₂
-        simp [H.expr_builtin, Builtin.eval, fn, h₂, Builtin.expr, Expr.eval]
-        simp [H₁.get!_builtin H]
-      rw [Map.get!_union_right # by simp [H.not_isBuiltin_of_mem h₁]]
-      rw [H.expr_of_mem_defs h₁]
-      rw [H.arity_of_mem_defs h₁] at h₂
-      have h₄ := @H₁.eval_eq
-      specialize @h₄ name d _ xs h₂
-      · rwa [Map.get?_ofList_eq_some_iff H.nodup_names]
-      convert h₄
-      simp [Prog.ext_iff]
-  ·
-    intro fs' h₁
-    specialize H₂ (fs' \ builtinFs) _
-    ·
-      sorry
-    subst H₂
-    symm; simp [Map.union_eq_self_left_iff]
-    rintro name b rfl
-    have h₂ := @h₁.eval_eq
-    specialize @h₂ b.name (by simp) (mkList b.arity id) _
-    ·
-      clear h₂
-      simp
-
-#check 0 #exit
-
-    -- constructor
-    -- · simp [H₁.keys_fs]
-    -- · intro name h₁ xs h₂
-    --   simp at h₁; rcases h₁ with ⟨b, rfl⟩ | ⟨d, h₁⟩
-    --   · apply H₁.eval_of_ne_arity (d := b.def) H.get?_builtin
-    --     contrapose! h₂
-    --     rw [h₂, Prog.arity_of_get? H.get?_builtin]
-    --   have h₃ := H.get?_of_mem_defs h₁
-    --   apply H₁.eval_of_ne_arity h₃
-    --   contrapose! h₂
-    --   rw [h₂, Prog.arity_of_get? h₃]
-    -- · intro name h₁ xs h₂
-    --   simp at h₁; rcases h₁ with ⟨b, rfl⟩ | ⟨d, h₁⟩
-    --   · have h₃ := @H₁.eval_eq b.name b.def H.get?_builtin xs
-    --     simp [Prog.arity_of_get? H.get?_builtin] at h₂
-    --     simp [h₂] at h₃
-    --     simp [H.expr_builtin]
-    --     convert h₃
-    --     simp [Prog.ext_iff]
-    --   simp [H.expr_of_mem_defs h₁]
-    --   simp [H.arity_of_mem_defs h₁] at h₂
-    --   convert @H₁.eval_eq name d (H.get?_of_mem_defs h₁) xs h₂
-    --   simp [Prog.ext_iff]
-
-#check 0 #exit
+  use H.compatible_fs_aux₁ H₁
+  intro fs' h
+  obtain ⟨fs', rfl, h₁⟩ := h.fs_eq_union
+  rw [Map.union_eq_union_iff_right # by simpa [IsBuiltin]]
+  rotate_left
+  · simp [IsBuiltin]; exact H₁.builtin_not_mem H
+  apply H₂; exact H.compatible_fs_aux₂ h h₁
 
 theorem WFDefs.wf {defs} (H : WFDefs defs) : (Prog.ofDefs defs).WF := by
   constructor
@@ -884,61 +486,18 @@ theorem WFDefs.wf {defs} (H : WFDefs defs) : (Prog.ofDefs defs).WF := by
 
 theorem wf_of_wfDefs {defs} (H : WFDefs defs) : (Prog.ofDefs defs).WF := H.wf
 
-@[simp, instance]
-theorem wf_progId : progId.WF := by
-  apply wf_of_wfDefs
-  constructor <;> try simp
-  use .ofList [(mainName, fn 1 λ xs => xs[0]!)]
-  split_ands
-  ·
-    dsimp
-    constructor
-    ·
-      simp
-
-#check 0 #exit
-
 @[simp]
 theorem Expr.run_call {prog fs args t xs} : (Expr.call t xs).eval prog fs args =
-t.f fs (xs.map λ x => x.eval prog fs args) := by
+fs.get! t (xs.map λ x => x.eval prog fs args) := by
   simp [eval]
-
-theorem not_wf_progLoop : ¬progLoop.WF := by
-  unfold progLoop exprLoop
-  rintro ⟨-, -, -, h⟩; contrapose! h; clear h
-  rw [not_exiu_iff_or]; right
-  use [fn 1 λ _ => 0], [fn 1 λ _ => 1]; unfold fn
-  simp; split_ands <;> try constructor <;> simp
-  apply ne_of_congr (· [0]); simp
 
 @[simp]
 theorem Prog.compatible_fs {prog : Prog} [H : prog.WF] : prog.Compatible prog.fs :=
   τ_spec H.exiu_compatible.exists
 
 @[simp]
-theorem eval_exprId {prog fs xs} : exprId.eval prog fs xs = xs[0]! := by
-  simp [exprId]
-
-@[simp]
-theorem run_progId {n} : progId.run n = n := by
-  simp [Prog.run, Prog.eval]; have h := @progId.compatible_fs.eval_eq
-  simp at h; specialize @h [n]; simpa using h
-
-@[simp]
-theorem Prog.hasTarget_builtin {prog : Prog} {bn} : prog.HasTarget (.builtin bn) := trivial
-
-@[simp]
-theorem Prog.hasTarget_custom {prog : Prog} {i} :
-prog.HasTarget (.custom i) ↔ i < prog.defs.length := by rfl
-
-@[simp] theorem Target.arity_builtin {bn} : arity (builtin bn) = bn.arity := rfl
-@[simp] theorem Target.f_builtin_succ {bn fs} : f (.builtin bn) fs = bn.f := rfl
-@[simp] theorem Builtin.f_succ : f .succ = (·[0]! + 1) := rfl
-@[simp] theorem Builtin.f_sub : f .sub = (λ xs => xs[0]! - xs[1]!) := rfl
-
-@[simp]
-theorem Expr.wf_call {prog t args n} : (call t args).WF prog n ↔ prog.HasTarget t ∧
-args.length = t.arity prog ∧ ∀ e ∈ args, e.WF prog n := by
+theorem Expr.wf_call {prog t args n} : (call t args).WF prog n ↔ prog.HasDef t ∧
+args.length = prog.arity t ∧ ∀ e ∈ args, e.WF prog n := by
   simp [WF]
 
 theorem Prog.fs_eq_of_compatible {prog : Prog} {fs} [hp : prog.WF]
@@ -948,5 +507,107 @@ theorem Prog.fs_eq_of_compatible {prog : Prog} {fs} [hp : prog.WF]
 instance {prog : Prog} {i} : Decidable # prog.HasDef i := by
   unfold Prog.HasDef; infer_instance
 
-instance {prog : Prog} {t} : Decidable # prog.HasTarget t := by
-  unfold Prog.HasTarget; cases t <;> infer_instance
+instance {prog : Prog} {t} : Decidable # prog.HasDef t := by
+  unfold Prog.HasDef; infer_instance
+
+-- example : ¬∀ {defs} (H : WFDefs defs),
+-- ∃! fs, (Prog.ofDefs defs).Compatible fs := by
+--   simp [not_exiu_iff]
+--   use [(mainName, ⟨1, exprId⟩)]
+--   split_ands
+--   ·
+--     constructor <;> simp
+--     use .ofList [(mainName, fn 1 (·[0]!))]
+--     simp
+--     split_ands
+--     ·
+--       constructor <;> simp [Map.get?_insert, Map.get!_eq_get!_get?, fn, exprId]
+--     ·
+--       intro fs
+--       rintro ⟨h₁, h₂, h₃⟩
+--       simp [Map.get?_insert, Map.get!_eq_get!_get?, exprId] at h₁ h₂ h₃
+--       simp [Map.ext_iff, Map.get?_insert]
+--       intro name
+--       rw! (castMode := .all) [eq_comm (a := mainName)]
+--       split_ifs with h₄
+--       rotate_left
+--       ·
+--         simp [←h₁] at h₄
+--         simpa
+--       subst h₄
+--       specialize h₁ mainName
+--       simp at h₁
+--       rw [Map.mem_iff_get?_eq_some] at h₁
+--       choose f h₁ using h₁
+--       ext xs
+--       simp [h₁]
+--       unfold fn
+--       simp
+--       revert xs
+--       simp
+--       ext xs
+--       split_ifs with h₄
+--       ·
+--         specialize h₃ h₄
+--         simp [h₁] at h₃
+--         rw [h₃]
+--       ·
+--         specialize h₂ h₄
+--         simp [h₁] at h₂
+--         rw [h₂]
+
+-----
+-----
+-----
+
+-- def exprId : Expr :=
+--   .arg 0
+-- 
+-- def exprLoop (name : String) : Expr :=
+--   .call name [.arg 0]
+-- 
+-- def progId : Prog :=
+--   .ofDefs [(mainName, ⟨1, exprId⟩)]
+-- 
+-- def progLoop : Prog :=
+--   .ofDefs [(mainName, ⟨1, exprLoop mainName⟩)]
+
+-- @[simp]
+-- theorem main_progId : progId.main = ⟨1, exprId⟩ := by
+--   simp [progId, Map.get!_insert]
+-- 
+-- @[simp]
+-- theorem main_progLoop : progLoop.main = ⟨1, exprLoop mainName⟩ := by
+--   simp [progLoop, Map.get!_insert]
+-- 
+-- @[simp] theorem wf_exprId {prog} : exprId.WF prog 1 := by simp [Expr.WF, exprId]
+-- @[simp] theorem wf_defId : (Def.mk 1 (.arg 0)).WF progId := wf_exprId
+
+-- theorem not_wf_progLoop : ¬progLoop.WF := by
+--   unfold progLoop exprLoop
+--   rintro ⟨-, -, -, h⟩; contrapose! h; clear h
+--   rw [not_exiu_iff_or]; right
+--   use [fn 1 λ _ => 0], [fn 1 λ _ => 1]; unfold fn
+--   simp; split_ands <;> try constructor <;> simp
+--   apply ne_of_congr (· [0]); simp
+-- 
+-- @[simp]
+-- theorem eval_exprId {prog fs xs} : exprId.eval prog fs xs = xs[0]! := by
+--   simp [exprId]
+-- 
+-- @[simp]
+-- theorem run_progId {n} : progId.run n = n := by
+--   simp [Prog.run, Prog.eval]; have h := @progId.compatible_fs.eval_eq
+--   simp at h; specialize @h [n]; simpa using h
+
+-- @[simp, instance]
+-- theorem wf_progId : progId.WF := by
+--   apply wf_of_wfDefs
+--   constructor <;> try simp
+--   use .ofList [(mainName, fn 1 λ xs => xs[0]!)]
+--   split_ands
+--   ·
+--     dsimp
+--     constructor
+--     ·
+--       simp
