Projects/Esolangs/Cornucopia/Prog1.lean
@@ -4,214 +4,214 @@ attribute [-simp] List.getElem!_eq_getElem?_getD
 
 namespace Esolangs.Cornucopia
 
-def refZero : Expr :=
-  .call (.custom 1) []
-
-def refOne : Expr :=
-  .call (.custom 2) []
-
-def exprZero : Expr :=
-  .call (.builtin .sub) [refZero, refZero]
-
-def exprOne : Expr :=
-  .call (.builtin .succ) [refZero]
-
-def exprNot : Expr :=
-  .call (.builtin .sub) [refOne, .arg 0]
-
-def exprBool : Expr :=
-  .call (.custom 3) [.call (.custom 3) [.arg 0]]
-
-def exprAdd : Expr :=
-  .call (.builtin .sub)
-  [ .call (.builtin .sub)
-    [ .call (.builtin .sub)
-      [ .call (.builtin .succ) [.call (.builtin .succ) [
-          .call (.custom 5)
-            [ .call (.builtin .sub) [.arg 0, refOne]
-            , .call (.builtin .sub) [.arg 1, refOne]
-            ]
-        ]]
-      , .call (.custom 3) [.arg 0]
-      ]
-    , .call (.custom 3) [.arg 1]
-    ]
-  , .call (.custom 5) [refZero, refZero]
-  ]
-
--- def refOneAlt : Expr :=
---   .call (.custom 6) []
+-- def refZero : Expr :=
+--   .call (.custom 1) []
 -- 
--- def exprOneAlt : Expr :=
+-- def refOne : Expr :=
+--   .call (.custom 2) []
+-- 
+-- def exprZero : Expr :=
+--   .call (.builtin .sub) [refZero, refZero]
+-- 
+-- def exprOne : Expr :=
+--   .call (.builtin .succ) [refZero]
+-- 
+-- def exprNot : Expr :=
+--   .call (.builtin .sub) [refOne, .arg 0]
+-- 
+-- def exprBool : Expr :=
+--   .call (.custom 3) [.call (.custom 3) [.arg 0]]
+-- 
+-- def exprAdd : Expr :=
 --   .call (.builtin .sub)
---   [ .call (.builtin .succ) [.custom 6]
+--   [ .call (.builtin .sub)
+--     [ .call (.builtin .sub)
+--       [ .call (.builtin .succ) [.call (.builtin .succ) [
+--           .call (.custom 5)
+--             [ .call (.builtin .sub) [.arg 0, refOne]
+--             , .call (.builtin .sub) [.arg 1, refOne]
+--             ]
+--         ]]
+--       , .call (.custom 3) [.arg 0]
+--       ]
+--     , .call (.custom 3) [.arg 1]
+--     ]
+--   , .call (.custom 5) [refZero, refZero]
 --   ]
-
-def exprMain₁ : Expr :=
-  exprId
-
-def prog₁ : Prog where
-  defs := [
-    ⟨1, exprMain₁⟩,
-    ⟨0, exprZero⟩,
-    ⟨0, exprOne⟩,
-    ⟨1, exprNot⟩,
-    ⟨1, exprBool⟩,
-    ⟨2, exprAdd⟩,
-  ]
-
-def prog₁FS : List (List ℕ → ℕ) :=
-  [ fn 1 λ xs => xs[0]!
-  , fn 0 λ _ => 0
-  , fn 0 λ _ => 1
-  , fn 1 λ xs => if xs[0]! = 0 then 1 else 0
-  , fn 1 λ xs => if xs[0]! = 0 then 0 else 1
-  , fn 2 λ xs => xs[0]! + xs[1]!
-  ]
-
--- #check 0 #exit
-
------
-
-@[simp]
-theorem wf_expr_prog₁_main₁ : exprMain₁.WF prog₁ 1 := by
-  simp [exprMain₁]
-
-@[simp]
-theorem wf_def_prog₁_main₁ : Def.WF prog₁ ⟨1, exprMain₁⟩ := by
-  simp [Def.WF]
-
--- #check 0 #exit
-
-theorem exprAdd_aux {f : ℕ → ℕ → ℕ} (h : ∀ x y, f x y = f (x - 1) (y - 1) + 2 -
-(if x = 0 then 1 else 0) - (if y = 0 then 1 else 0) - f 0 0) : f = (· + ·) := by
-  ext x y
-  have h₁ : f 0 0 = 0
-  · specialize h 0 0
-    simpa using h
-  induction x generalizing y
-  · specialize h 0
-    simp at h
-    induction y
-    · specialize h 0
-      simpa using h
-    nm y ih
-    specialize h (y + 1)
-    simp_all
-  nm x ih
-  specialize h (x + 1) y
-  simp_all
-  specialize ih (y + 1)
-  grind
-
--- #check 0 #exit
-
-@[simp] theorem length_defs_prog₁ : prog₁.defs.length = 6 := rfl
-
-@[simp] theorem prog₁_arity_0 : prog₁.arity 0 = 1 := rfl
-@[simp] theorem prog₁_arity_1 : prog₁.arity 1 = 0 := rfl
-@[simp] theorem prog₁_arity_2 : prog₁.arity 2 = 0 := rfl
-@[simp] theorem prog₁_arity_3 : prog₁.arity 3 = 1 := rfl
-@[simp] theorem prog₁_arity_4 : prog₁.arity 4 = 1 := rfl
-@[simp] theorem prog₁_arity_5 : prog₁.arity 5 = 2 := rfl
-
-@[simp]
-theorem wf_prog₁_refZero {n} : refZero.WF prog₁ n := by
-  simp [refZero]
-
-@[simp]
-theorem wf_expr_prog₁_exprZero {n} : exprZero.WF prog₁ n := by
-  simp [exprZero]
-
-@[simp]
-theorem wf_prog₁_refOne {n} : refOne.WF prog₁ n := by
-  simp [refOne]
-
-@[simp]
-theorem wf_expr_prog₁_exprOne {n} : exprOne.WF prog₁ n := by
-  simp [exprOne]
-
-@[simp]
-theorem wf_expr_prog₁_exprNot {n} : exprNot.WF prog₁ n ↔ 1 ≤ n := by
-  simp [exprNot]; omega
-
-@[simp]
-theorem wf_expr_prog₁_exprBool {n} : exprBool.WF prog₁ n ↔ 1 ≤ n := by
-  simp [exprBool]; omega
-
-@[simp]
-theorem wf_expr_prog₁_exprAdd {n} : exprAdd.WF prog₁ n ↔ 2 ≤ n := by
-  simp [exprAdd]; omega
-
--- #check 0 #exit
-
-@[simp]
-theorem compatible_prog₁_prog₁FS : prog₁.Compatible prog₁FS := by
-  unfold prog₁FS; constructor <;> simp
-  all_goals
-    intro i h xs h₁
-    obtain rfl | rfl | rfl | rfl | rfl | rfl :
-      i = 0 ∨ i = 1 ∨ i = 2 ∨ i = 3 ∨ i = 4 ∨ i = 5 := by omega
-  iterate 6 simp at h₁; simp [fn] <;> try grind
-  all_goals nth_rw 1 [prog₁]; (try simp at h₁); simp [fn, h₁]
-  · simp [exprMain₁, exprId]
-  · simp [exprZero]
-  · simp [exprOne, refZero, fn]
-  · simp [exprNot, refOne, fn]; grind
-  · simp [exprBool, fn]; grind
-  · simp [exprAdd, fn]; rw! [xs.eq_getElem_of_length_eq_two h₁]
-    simp; generalize xs[0] = x; generalize xs[1] = y; clear h₁ xs
-    simp [refOne, refZero, fn]; cases x; cases y <;> rfl; nm x
-    simp; cases y; rfl; nm y; simp; omega
-
-@[simp, instance]
-theorem wf_prog₁ : prog₁.WF := by
-  constructor; rintro ⟨⟩; rfl; nth_rw 1 [prog₁]; simp
-  use prog₁FS, (by simp); unfold prog₁FS
-  rintro fs ⟨h₁, h₂, h₃⟩; simp at h₁ h₂ h₃
-  have h_zero : fs[1]! [] = 0
-  · specialize @h₃ 1 (by omega) [] (by simp)
-    simp [prog₁, exprZero] at h₃; exact h₃
-  have h_one : fs[2]! [] = 1
-  · specialize @h₃ 2 (by omega) [] (by simp)
-    simp [prog₁, exprOne, refZero] at h₃; grind
-  have h_not : ∀ ⦃x⦄, fs[3]! [x] = if x = 0 then 1 else 0
-  · intro x; specialize @h₃ 3 (by omega) [x] (by simp)
-    simp [prog₁, exprNot, refOne] at h₃; grind
-  have h_bool : ∀ ⦃x⦄, fs[4]! [x] = if x = 0 then 0 else 1
-  · intro x; specialize @h₃ 4 (by omega) [x] (by simp)
-    simp [prog₁, exprBool] at h₃; grind
-  have h_add : ∀ ⦃x y⦄, fs[5]! [x, y] = x + y
-  · intro x y; specialize @h₃ 5 (by omega)
-    simp [prog₁, exprAdd, refOne, refZero] at h₃
-    simp [h_zero, h_one, h_not] at h₃
-    replace h₃ : ∀ x y, fs[5]! [x, y] = fs[5]! [x - 1, y - 1] + 2 -
-      (if x = 0 then 1 else 0) - (if y = 0 then 1 else 0) - fs[5]! [0, 0]
-    · intro x y; specialize @h₃ [x, y]; simp at h₃; omega
-    have h₄ := exprAdd_aux (f := λ x y => fs[5]! [x, y]) (by grind); grind
-  rw [List.ext_getElem!_iff]; simp [h₁]; intro i h₄; ext xs
-  specialize @h₂ i (by omega); specialize @h₃ i (by omega)
-  specialize @h₂ xs; specialize @h₃ xs
-  obtain rfl | rfl | rfl | rfl | rfl | rfl :
-    i = 0 ∨ i = 1 ∨ i = 2 ∨ i = 3 ∨ i = 4 ∨ i = 5 := by omega
-  all_goals simp [prog₁, fn] at h₂ h₃ ⊢
-  · split_ifs with H
-    · specialize h₃ H; simp [exprMain₁, exprId] at h₃; grind
-    · specialize h₂ H; grind
-  · simp [exprZero] at h₃; grind
-  · simp [exprOne] at h₂ h₃; grind
-  · simp [exprNot, refOne] at h₂ h₃; grind
-  · simp [exprBool] at h₂ h₃; grind
-  · simp [exprAdd, refOne, refZero] at h₂ h₃; grind
-
-@[simp]
-theorem fs_prog₁ : prog₁.fs = prog₁FS :=
-  Prog.fs_eq_of_compatible compatible_prog₁_prog₁FS
-
-@[simp]
-theorem eval_prog₁ {i xs} : prog₁.eval i xs = prog₁FS[i]! xs := by
-  simp [Prog.eval]
-
-@[simp]
-theorem run_prog₁ {x} : prog₁.run x = x := by
-  simp [Prog.run, Prog.eval, prog₁FS, fn]
+-- 
+-- -- def refOneAlt : Expr :=
+-- --   .call (.custom 6) []
+-- -- 
+-- -- def exprOneAlt : Expr :=
+-- --   .call (.builtin .sub)
+-- --   [ .call (.builtin .succ) [.custom 6]
+-- --   ]
+-- 
+-- def exprMain₁ : Expr :=
+--   exprId
+-- 
+-- def prog₁ : Prog where
+--   defs := [
+--     ⟨1, exprMain₁⟩,
+--     ⟨0, exprZero⟩,
+--     ⟨0, exprOne⟩,
+--     ⟨1, exprNot⟩,
+--     ⟨1, exprBool⟩,
+--     ⟨2, exprAdd⟩,
+--   ]
+-- 
+-- def prog₁FS : List (List ℕ → ℕ) :=
+--   [ fn 1 λ xs => xs[0]!
+--   , fn 0 λ _ => 0
+--   , fn 0 λ _ => 1
+--   , fn 1 λ xs => if xs[0]! = 0 then 1 else 0
+--   , fn 1 λ xs => if xs[0]! = 0 then 0 else 1
+--   , fn 2 λ xs => xs[0]! + xs[1]!
+--   ]
+-- 
+-- -- #check 0 #exit
+-- 
+-- -----
+-- 
+-- @[simp]
+-- theorem wf_expr_prog₁_main₁ : exprMain₁.WF prog₁ 1 := by
+--   simp [exprMain₁]
+-- 
+-- @[simp]
+-- theorem wf_def_prog₁_main₁ : Def.WF prog₁ ⟨1, exprMain₁⟩ := by
+--   simp [Def.WF]
+-- 
+-- -- #check 0 #exit
+-- 
+-- theorem exprAdd_aux {f : ℕ → ℕ → ℕ} (h : ∀ x y, f x y = f (x - 1) (y - 1) + 2 -
+-- (if x = 0 then 1 else 0) - (if y = 0 then 1 else 0) - f 0 0) : f = (· + ·) := by
+--   ext x y
+--   have h₁ : f 0 0 = 0
+--   · specialize h 0 0
+--     simpa using h
+--   induction x generalizing y
+--   · specialize h 0
+--     simp at h
+--     induction y
+--     · specialize h 0
+--       simpa using h
+--     nm y ih
+--     specialize h (y + 1)
+--     simp_all
+--   nm x ih
+--   specialize h (x + 1) y
+--   simp_all
+--   specialize ih (y + 1)
+--   grind
+-- 
+-- -- #check 0 #exit
+-- 
+-- @[simp] theorem length_defs_prog₁ : prog₁.defs.length = 6 := rfl
+-- 
+-- @[simp] theorem prog₁_arity_0 : prog₁.arity 0 = 1 := rfl
+-- @[simp] theorem prog₁_arity_1 : prog₁.arity 1 = 0 := rfl
+-- @[simp] theorem prog₁_arity_2 : prog₁.arity 2 = 0 := rfl
+-- @[simp] theorem prog₁_arity_3 : prog₁.arity 3 = 1 := rfl
+-- @[simp] theorem prog₁_arity_4 : prog₁.arity 4 = 1 := rfl
+-- @[simp] theorem prog₁_arity_5 : prog₁.arity 5 = 2 := rfl
+-- 
+-- @[simp]
+-- theorem wf_prog₁_refZero {n} : refZero.WF prog₁ n := by
+--   simp [refZero]
+-- 
+-- @[simp]
+-- theorem wf_expr_prog₁_exprZero {n} : exprZero.WF prog₁ n := by
+--   simp [exprZero]
+-- 
+-- @[simp]
+-- theorem wf_prog₁_refOne {n} : refOne.WF prog₁ n := by
+--   simp [refOne]
+-- 
+-- @[simp]
+-- theorem wf_expr_prog₁_exprOne {n} : exprOne.WF prog₁ n := by
+--   simp [exprOne]
+-- 
+-- @[simp]
+-- theorem wf_expr_prog₁_exprNot {n} : exprNot.WF prog₁ n ↔ 1 ≤ n := by
+--   simp [exprNot]; omega
+-- 
+-- @[simp]
+-- theorem wf_expr_prog₁_exprBool {n} : exprBool.WF prog₁ n ↔ 1 ≤ n := by
+--   simp [exprBool]; omega
+-- 
+-- @[simp]
+-- theorem wf_expr_prog₁_exprAdd {n} : exprAdd.WF prog₁ n ↔ 2 ≤ n := by
+--   simp [exprAdd]; omega
+-- 
+-- -- #check 0 #exit
+-- 
+-- @[simp]
+-- theorem compatible_prog₁_prog₁FS : prog₁.Compatible prog₁FS := by
+--   unfold prog₁FS; constructor <;> simp
+--   all_goals
+--     intro i h xs h₁
+--     obtain rfl | rfl | rfl | rfl | rfl | rfl :
+--       i = 0 ∨ i = 1 ∨ i = 2 ∨ i = 3 ∨ i = 4 ∨ i = 5 := by omega
+--   iterate 6 simp at h₁; simp [fn] <;> try grind
+--   all_goals nth_rw 1 [prog₁]; (try simp at h₁); simp [fn, h₁]
+--   · simp [exprMain₁, exprId]
+--   · simp [exprZero]
+--   · simp [exprOne, refZero, fn]
+--   · simp [exprNot, refOne, fn]; grind
+--   · simp [exprBool, fn]; grind
+--   · simp [exprAdd, fn]; rw! [xs.eq_getElem_of_length_eq_two h₁]
+--     simp; generalize xs[0] = x; generalize xs[1] = y; clear h₁ xs
+--     simp [refOne, refZero, fn]; cases x; cases y <;> rfl; nm x
+--     simp; cases y; rfl; nm y; simp; omega
+-- 
+-- @[simp, instance]
+-- theorem wf_prog₁ : prog₁.WF := by
+--   constructor; rintro ⟨⟩; rfl; nth_rw 1 [prog₁]; simp
+--   use prog₁FS, (by simp); unfold prog₁FS
+--   rintro fs ⟨h₁, h₂, h₃⟩; simp at h₁ h₂ h₃
+--   have h_zero : fs[1]! [] = 0
+--   · specialize @h₃ 1 (by omega) [] (by simp)
+--     simp [prog₁, exprZero] at h₃; exact h₃
+--   have h_one : fs[2]! [] = 1
+--   · specialize @h₃ 2 (by omega) [] (by simp)
+--     simp [prog₁, exprOne, refZero] at h₃; grind
+--   have h_not : ∀ ⦃x⦄, fs[3]! [x] = if x = 0 then 1 else 0
+--   · intro x; specialize @h₃ 3 (by omega) [x] (by simp)
+--     simp [prog₁, exprNot, refOne] at h₃; grind
+--   have h_bool : ∀ ⦃x⦄, fs[4]! [x] = if x = 0 then 0 else 1
+--   · intro x; specialize @h₃ 4 (by omega) [x] (by simp)
+--     simp [prog₁, exprBool] at h₃; grind
+--   have h_add : ∀ ⦃x y⦄, fs[5]! [x, y] = x + y
+--   · intro x y; specialize @h₃ 5 (by omega)
+--     simp [prog₁, exprAdd, refOne, refZero] at h₃
+--     simp [h_zero, h_one, h_not] at h₃
+--     replace h₃ : ∀ x y, fs[5]! [x, y] = fs[5]! [x - 1, y - 1] + 2 -
+--       (if x = 0 then 1 else 0) - (if y = 0 then 1 else 0) - fs[5]! [0, 0]
+--     · intro x y; specialize @h₃ [x, y]; simp at h₃; omega
+--     have h₄ := exprAdd_aux (f := λ x y => fs[5]! [x, y]) (by grind); grind
+--   rw [List.ext_getElem!_iff]; simp [h₁]; intro i h₄; ext xs
+--   specialize @h₂ i (by omega); specialize @h₃ i (by omega)
+--   specialize @h₂ xs; specialize @h₃ xs
+--   obtain rfl | rfl | rfl | rfl | rfl | rfl :
+--     i = 0 ∨ i = 1 ∨ i = 2 ∨ i = 3 ∨ i = 4 ∨ i = 5 := by omega
+--   all_goals simp [prog₁, fn] at h₂ h₃ ⊢
+--   · split_ifs with H
+--     · specialize h₃ H; simp [exprMain₁, exprId] at h₃; grind
+--     · specialize h₂ H; grind
+--   · simp [exprZero] at h₃; grind
+--   · simp [exprOne] at h₂ h₃; grind
+--   · simp [exprNot, refOne] at h₂ h₃; grind
+--   · simp [exprBool] at h₂ h₃; grind
+--   · simp [exprAdd, refOne, refZero] at h₂ h₃; grind
+-- 
+-- @[simp]
+-- theorem fs_prog₁ : prog₁.fs = prog₁FS :=
+--   Prog.fs_eq_of_compatible compatible_prog₁_prog₁FS
+-- 
+-- @[simp]
+-- theorem eval_prog₁ {i xs} : prog₁.eval i xs = prog₁FS[i]! xs := by
+--   simp [Prog.eval]
+-- 
+-- @[simp]
+-- theorem run_prog₁ {x} : prog₁.run x = x := by
+--   simp [Prog.run, Prog.eval, prog₁FS, fn]
